only pull in trait functions

Source/DafnyCore/Verifier/Translator.ClassMembers.cs
@@ -1098,7 +1098,9 @@ namespace Microsoft.Dafny {
       }
 
       // useViaContext: fh < FunctionContextHeight
-      Boogie.Expr useViaContext = Boogie.Expr.Lt(Boogie.Expr.Literal(forModule.CallGraph.GetSCCRepresentativePredecessorCount(f)), etran.FunctionContextHeight());
+      Boogie.Expr useViaContext = !InVerificationScope(overridingFunction)
+        ? Boogie.Expr.True
+        : Boogie.Expr.Lt(Boogie.Expr.Literal(forModule.CallGraph.GetSCCRepresentativePredecessorCount(f)), etran.FunctionContextHeight());
 
       // useViaCanCall: C.F#canCall(args)
       Bpl.IdentifierExpr canCallFuncID = new Bpl.IdentifierExpr(overridingFunction.tok, overridingFunction.FullSanitizedName + "#canCall", Bpl.Type.Bool);
